Refactor: remove all uses of All2_aux

sepcomp/seq_lemmas.v
@@ -9,24 +9,19 @@ Fixpoint All T P (l : seq T) :=
     | a :: l' => [/\ P a & All P l']
   end.
 
-Fixpoint All2_aux U T (P : U -> T -> Prop) (a : U) (l : seq T) :=
-  if l is [:: a' & l'] then
-    [/\ P a a' & All2_aux P a l']
-  else True. 
-
 Fixpoint All2 T (P : T -> T -> Prop) (l : seq T) :=
-  if l is [:: a & l'] then [/\ All2_aux P a l' & All2 P l']
+  if l is [:: a & l'] then [/\ All (P a) l' & All2 P l']
   else True.
 
 Lemma All2_cons T P (a : T) (l : seq T) :
-  All2 P [:: a & l] <-> [/\ All2_aux P a l & All2 P l].
+  All2 P [:: a & l] <-> [/\ All (P a) l & All2 P l].
 Proof. by split=> /= => [][]A B; split. Qed.
 
-Lemma All2_aux_sub T (P P' : T -> T -> Prop) a l :
-  All2_aux P a l -> (forall a a', P a a' -> P' a a') -> All2_aux P' a l.
+Lemma All_sub T (P P' : T -> Prop) l :
+  All P l -> (forall a, P a -> P' a) -> All P' l.
 Proof.
 move=> A B; move: A; elim: l=> // a' l' IH /= []C D; split.
-by apply: (B _ _ C).
+by apply: (B _ C).
 by apply: IH.
 Qed.
 
@@ -34,7 +29,7 @@ Lemma All2_sub T (P P' : T -> T -> Prop) l :
   All2 P l -> (forall a a', P a a' -> P' a a') -> All2 P' l.
 Proof.
 move=> A B; move: A; elim: l=> // a l' IH /= []C D; split.
-by apply: (All2_aux_sub C).
+by apply: (All_sub C); apply: B.
 by apply: (IH D).
 Qed.
 
@@ -47,31 +42,21 @@ move=> /= => [][][]A B []C D HC; split=> //.
 by split=> //; apply: (HC _ _ A).
 Qed.
 
-Lemma All2_aux_comp T U (P : T -> T -> Prop) (f : U -> T) a l :
-  All2_aux (fun a b : U => P (f a) (f b)) a l <-> 
-  All2_aux P (f a) (map f l).
+Lemma All_comp T U (P : T -> Prop) (f : U -> T) l :
+  All (P \o f) l <-> All P (map f l).
 Proof.
-move: a; elim: l=> // a' l' IH a''; split.
-by move=> /= []A B; split=> //; rewrite -IH.
-by move=> /= []A B; split=> //; rewrite IH.
-Qed.
-
-Lemma All2_aux_comp2 T U W (P : U -> W -> Prop) (f : T -> U) a l :
-  All2_aux P (f a) l <-> All2_aux (P \o f) a l.
-Proof.
-move: a; elim: l=> // a' l' IH a''; split.
+elim: l=> // a' l' IH; split.
 by move=> /= []A B; split=> //; rewrite -IH.
 by move=> /= []A B; split=> //; rewrite IH.
 Qed.
 
 Lemma All2_comp T U (P : T -> T -> Prop) (f : U -> T) l :
-  All2 (fun a b => P (f a) (f b)) l <-> 
-  (All2 P \o map f) l.
+  All2 (fun a b => P (f a) (f b)) l <-> (All2 P \o map f) l.
 Proof.
 elim: l=> // a l' IH; split.
-move=> /= []A B; split; first by rewrite -All2_aux_comp. 
+move=> /= []A B; split; first by rewrite -All_comp. 
 by case: IH; move/(_ B)=> C _; apply: C.
-move=> /= []A B; split; first by rewrite All2_aux_comp.
+move=> /= []A B; split; first by rewrite All_comp.
 by case: IH=> _; move/(_ B).
 Qed.
 
